\documentclass[12pt]{article}
\usepackage[margin=1in]{geometry} 
\usepackage{amsmath,amsthm,amssymb}
\parindent 0px
\begin{document}
 Abhilash Rapolu \hfill {\Large ASSIGNMENT 1} \hfill \today
\\EE23BTECH11052
\subsection*{Question 11.9.2.10}
 If the sum of first $p$ terms of an A.P. is equal to the sum of the first $q$ terms, then
 find the sum of the first $(p + q)$ terms?

\subsection*{Solution:}
The sum of first $p$ terms of an arithmetic progression (A.P) is given by
\bgroup \obeylines
Let $a_1$ be the first term which is $a_0+d$
$$s_p =\frac{q}{2}[2a_1+(q-1)d]$$
$$s_p =\frac{q}{2}[2a_0+(q+1)d]$$
If $s_p$=$s_q$,then:
$$\frac{p}{2}[2a_0+(p+1)d]=\frac{q}{2}[2a_0+(q+1)d]$$
simplifying the equation we get:
\egroup
\begin{equation}
(p)*(2a_0+pd+d)=(q)*(2a_0+qd+d)
\end{equation}
\begin{equation}
2a_0p+(p^2)*d+pd=2a_0q+(q^2)*d+qd
\end{equation}
\begin{equation}
2a_0(p-q)+(p-q)(p+q)*d+(p-q)*d=0
\end{equation}
\begin{equation}
(p-q)[2a_0+(p+q)*d+d]=0
\end{equation}
since $p$ and $q$ are not equal.We can eliminate the term $(p-q)$
\begin{equation}
2a_0+(p+q)*d+d=0
\end{equation}
 Sum of the first $p+q$
$$S_{p+q}=\frac{p+q}{2}[2a_0+(p+q+1)*d]$$
\\As we have seen in the equation $(5)$ $2a_0+(p+q)*d+d=0$ is $0$.
 Therefore $S_{p+q}$ is $0$.
\end{document}
